BoogieLang/MapExample.thy
@@ -1,0 +1,270 @@
+section \<open>Instantiation Example for MapV\<close>
+
+theory MapExample
+  imports Semantics VCExprHelper Map3Semantics
+begin
+
+(* MapV datatype *)
+value "IntV 2 :: unit valn"
+
+abbreviation IntV0 where "IntV0 i \<equiv> LitV0 (LInt i)"
+abbreviation TT where "TT \<equiv> TPrim TInt"  (* convenience for testing purposes *)
+
+abbreviation m11 :: "'a val1" where "m11 \<equiv> FunL (undefined(IntV0 3 := Inr (IntV0 2))) TT TT"
+abbreviation m14 :: "'a valn" where "m14 \<equiv> MapV (Inr (Inr m11))"
+
+abbreviation m22 :: "'a val2" where "m22 \<equiv> FunL (undefined(Inl m11 := Inr (Inr (IntV0 4)))) TT TT"
+abbreviation m24 :: "'a valn" where "m24 \<equiv> MapV (Inr (Inl m22))"
+
+abbreviation m33 :: "'a val3" where "m33 \<equiv> FunL (undefined(Inl m22 := Inr (Inr (Inr (IntV0 6))))) TT TT"
+abbreviation m34 :: "'a valn" where "m34 \<equiv> MapV (Inl m33)"
+
+abbreviation mg3 :: "'a val3" where "mg3 \<equiv> FunL (undefined(Inl m22 := Inr (Inr (Inl  m11)))) (TMap TT TT) TT"
+abbreviation mg4 :: "'a valn" where "mg4 \<equiv> MapV (Inl mg3)"
+
+abbreviation ms3 :: "'a val3" where "ms3 \<equiv> FunL (undefined(Inr (Inr (IntV0 3)) := Inl m33)) TT (TMap TT  (TPrim TInt))"
+abbreviation ms4 :: "'a valn" where "ms4 \<equiv> MapV (Inl ms3)"
+
+(* type *)
+lemma map_level_gt_0: "tmap_lvl (TMap tv tk) \<ge> 1" by auto
+
+(* select *)
+lemma "selectImpl mg4 m24 = m14" by simp
+
+(* store *)
+lemma "type_of_val (LitV (LInt 42)) = TT" by simp
+lemma "ran_ty mg4 = TT" by simp
+lemma "selectImpl (storeImpl mg4 m24 (LitV (LInt 42))) m24
+  = (LitV (LInt 42))" by simp
+
+
+subsubsection \<open>Proving well formdness of a simple map\<close>
+fun toVal0 :: "'a valn \<Rightarrow> 'a val0" where "toVal0 (LitV l) = LitV0 l" | "toVal0 _ = undefined"
+fun fAdd1 where "fAdd1 (IntV0 x) = Inr (IntV0 (x+1))" | "fAdd1 _ = Inr (toVal0 (val_of_type (TT)))"
+abbreviation mAdd1 :: "'a::absval val1" where "mAdd1 \<equiv> FunL fAdd1 (TPrim TInt) (TPrim TInt)"
+abbreviation vAdd1 :: "'a::absval valn" where "vAdd1 \<equiv> MapV (Inr (Inr mAdd1))"
+
+lemma wfvotTT: "(type_of_val ((val_of_type TT)::'a::absval valn) = TT \<and> wf ((val_of_type TT)::'a::absval valn))"
+  by (metis (mono_tags, lifting) someI_ex tint_intv type_of_lit.simps(2) type_of_val.simps(1)
+      val_of_type.simps wfLitV)
+
+lemma mAdd1Typesafe:
+  shows "type_of_val (selectImpl vAdd1 k) = (TPrim TInt)"
+  apply (cases k rule: toVal3210.cases)
+  apply (metis (no_types, lifting) fAdd1.elims int_inverse_3 selectImpl.simps selectImplAux.simps(3)
+      toVal0.simps(1) toVal3210.simps(1,3) type_of_lit.simps(2) type_of_val.simps(1) val3ToValn.simps(1)
+      wfvotTT)
+  using wfvotTT tint_intv
+  apply (metis (no_types, opaque_lifting) fAdd1.simps(4) selectImpl.simps selectImplAux.simps(3)
+      toVal0.simps(1) toVal3210.simps(1,3) val3ToValn.simps(2) valBij valBij2)
+  apply (metis dom_ty.elims fst_conv mapval_ty_eq_ty321 selectImpl.simps selectImplAux.simps(11)
+      toVal3210.simps(3) ty.sel(5) ty321.simps(1) tyL.simps type_of_val.simps(3) valBij2 wfvotTT)
+  apply (metis dom_ty.elims fst_conv mapval_ty_eq_ty321 selectImpl.simps selectImplAux.simps(10)
+      toVal3210.simps(3,4) ty.sel(5) ty321.simps(1) tyL.simps type_of_val.simps(3) valBij2 wfvotTT)
+  apply (metis dom_ty.elims fst_conv mapval_ty_eq_ty321 selectImpl.simps selectImplAux.simps(09)
+      toVal3210.simps(3,5) ty.sel(5) ty321.simps(1) tyL.simps type_of_val.simps(3) valBij2 wfvotTT)
+  done
+
+(* TODO: more general *)
+lemma votTTpreserved: "val3ToValn (Inr (Inr (Inr (toVal0 (val_of_type (TT)))))) = (val_of_type (TT))"
+  by (metis int_inverse_3 toVal0.simps(1) val3ToValn.simps(1) wfvotTT)
+
+lemma vAdd1defualt: "(\<not>wf k \<or> type_of_val k \<noteq> dom_ty vAdd1) \<Longrightarrow> (selectImpl vAdd1 k) = val_of_type (ran_ty vAdd1)"
+  apply (cases "k" rule: toVal3210.cases; cases "type_of_val k"; simp) 
+      apply (rename_tac v t, case_tac v; simp) using votTTpreserved apply fastforce
+  using wfLitV wfAbsV toVal3210_inj valBij apply blast
+  using votTTpreserved apply auto[1]
+  using votTTpreserved apply auto[1]
+  using wfLitV wfAbsV toVal3210_inj valBij apply blast+
+  done
+
+lemma vAdd1wfSelect: "wf (selectImpl vAdd1 k)"
+  using mAdd1Typesafe tint_intv wf.simps by blast
+
+lemma wf_vAdd1: "wf vAdd1"
+  using vAdd1wfSelect vAdd1defualt mAdd1Typesafe wfMapV[of vAdd1] by auto
+
+
+subsubsection \<open>Well formdness of a higher order map\<close>
+
+locale valoftype =
+  assumes VOT: "\<And>t. tmap_lvl t \<le> 3 \<Longrightarrow> closed t \<Longrightarrow> (type_of_val ((val_of_type t)::'a::absval valn) = t \<and> wf ((val_of_type t)::'a::absval valn))"
+begin
+
+fun toVal1 :: "'a valn \<Rightarrow> 'a val1" where "toVal1 (MapV (Inr (Inr m))) = m" | "toVal1 _ = undefined"
+fun val0Of10 :: "'a val1 + 'a val0 \<Rightarrow> 'a val0" where "val0Of10 (Inr v0) = v0" | "val0Of10 _ = undefined"
+abbreviation TMII where "TMII \<equiv> TMap (TPrim TInt) (TPrim TInt)"
+fun compint where 
+    "compint g f (IntV0 x) =  (g (val0Of10 (f (IntV0 x))))"
+    | "compint g f _ =  Inr (toVal0 (val_of_type (TT)))"
+fun hof where 
+  "hof (Inl (FunL f tk tv)) =
+    (if (tk, tv) = (TT, TT) \<and> wf (MapV (Inr (Inr (FunL f tk tv))))
+        then Inr (Inl (FunL (compint fAdd1 f) TT TT))
+        else Inr (Inl (toVal1 (val_of_type (TMII)))))"
+  | "hof _ = Inr (Inl (toVal1 (val_of_type (TMII))))"
+abbreviation hom :: "'a::absval val2" where "hom \<equiv> FunL hof TMII TMII"
+abbreviation homV :: "'a::absval valn" where "homV \<equiv> MapV (Inr (Inl hom))"
+
+lemma "wf_ty homV" by auto
+
+lemma "ran_ty homV = TMII" by simp
+
+lemma "dom_ty homV = TMII" by simp
+
+lemma "type_of_val k = TMII \<longrightarrow> (\<exists>k'. k = MapV k')" apply (cases k) by auto
+
+lemma kTMII:
+  assumes "wf_ty k"
+  assumes "type_of_val k = TMII"
+  shows "\<exists>f. k = MapV (Inr (Inr (FunL f TT TT)))"
+proof -
+  have "tmap_lvl (type_of_val k) = 1" using assms by simp
+  then obtain k' where "toVal3210 k = Inr (Inr (Inl k'))" using C1Inrrl assms by blast
+  then have K: "k = MapV (Inr (Inr k'))" using toVal3210.elims by auto
+  then have "wf_L 1 k'" using assms by force
+  then show ?thesis
+    apply (cases k')
+    using K assms(2) by auto
+qed
+
+lemma validClosedTMII: "tmap_lvl (TMap TT TT) \<le> 3 \<and> closed (TMap TT TT)" by simp
+
+lemma homvotdef: "tyL (toVal1 (val_of_type (TMap TT TT))) = (TT, TT)" using VOT
+  by (metis kTMII toVal1.simps(1) tyL.simps validClosedTMII wf.simps
+      wf_ty.simps(1,2))
+
+
+lemma votTMIIpreserved: "val3ToValn (Inr (Inr (Inl (toVal1 (val_of_type (TMII)))))) = (val_of_type (TMII))"
+  by (metis VOT kTMII toVal1.simps(1) val3ToValn.simps(3) validClosedTMII wf.simps
+      wf_ty.simps(1,2))
+
+
+lemma wff: "type_of_val (selectImpl homV k) = TMII"
+  apply (case_tac k rule: ValnCases; (simp add: valBij2))
+    using homvotdef VOT by auto
+
+lemma compwf:
+  assumes "a = (MapV (Inr (Inr (FunL f TT TT))))"
+  assumes "b = (MapV (Inr (Inr (FunL (compint fAdd1 f) TT TT))))"
+  assumes "wf a"
+  shows "wf b"
+proof -
+  have wft: "wf_ty b" by (simp add: assms(2))
+
+  have wf1: "\<forall>k. wf (selectImpl b k)"
+    apply rule
+    apply (case_tac k rule: toVal3210.cases; (simp add: assms))
+    apply (rename_tac v, case_tac v; (simp add: assms))
+    apply (metis val_of_type.simps votTTpreserved wfvotTT)
+    apply (metis fAdd1.elims val3ToValn.simps(1) votTTpreserved wfLitV wfvotTT)
+    apply (metis val_of_type.simps votTTpreserved wfvotTT)
+    apply (metis toVal3210.simps(1) val0.exhaust val3ToValn.simps(2) valBij2 wfAbsV
+        wfLitV)
+    apply (metis valBij2 val_of_type.simps wfvotTT)+
+    done
+  have KTT: "dom_ty b = TT" by (simp add: assms(2))
+  have wf2: "\<forall>k. (\<not>wf k \<or> type_of_val k \<noteq> dom_ty b) \<longrightarrow> (selectImpl b k) = val_of_type (ran_ty b)"
+  proof (rule) fix k
+    show "(\<not>wf k \<or> type_of_val k \<noteq> dom_ty b) \<longrightarrow> (selectImpl b k) = val_of_type (ran_ty b)"
+    proof (cases k rule: toVal3210.cases)
+      case (1 v)
+      then show ?thesis apply (cases v)
+        using assms(2) votTTpreserved apply auto[1]
+        apply (simp add: KTT wfLitV)
+        using assms(2) votTTpreserved apply auto
+        done
+    next
+      case (2 v)
+      then show ?thesis
+        using assms(2) votTTpreserved by auto
+    qed (auto simp add: assms valBij2)
+  qed
+    
+  have wf3: "\<forall>k. type_of_val (selectImpl b k) = ran_ty b"
+    apply rule
+    apply (case_tac k rule: toVal3210.cases; (simp add: assms))
+    apply (rename_tac v, case_tac v; simp)
+    apply (metis val_of_type.simps votTTpreserved wfvotTT)
+    apply (metis (no_types, lifting) fAdd1.elims type_of_lit.simps(2) type_of_val.simps(1)
+        val3ToValn.simps(1) votTTpreserved wfvotTT)
+    apply (metis val_of_type.simps votTTpreserved wfvotTT)
+    apply (metis val_of_type.simps votTTpreserved wfvotTT)
+    apply (metis valBij2 val_of_type.simps wfvotTT)+
+    done
+
+  have wf2: "\<forall>k. (\<not>wf k \<or> type_of_val k \<noteq> dom_ty b) \<longrightarrow> (selectImpl b k) = val_of_type (ran_ty b)"
+    apply rule
+    apply (case_tac k rule: toVal3210.cases; (simp add: assms valBij2))
+        apply (rename_tac v, case_tac v; simp)
+    using votTTpreserved apply fastforce
+    using wfLitV apply blast
+    using votTTpreserved apply fastforce+
+    done
+
+  show ?thesis using wft wf1 wf2 wf3 wfMapV by simp
+qed
+
+
+lemma vhomVwfSelect: "wf (selectImpl homV k)"
+  apply (cases k rule: toVal3210.cases; simp)
+  using VOT votTMIIpreserved apply auto[1]
+  using VOT votTMIIpreserved apply auto[1]
+    apply (rename_tac m, case_tac m)
+    using VOT validClosedTMII val_of_type.simps
+    apply (simp add: valBij2)
+    using valoftype.compwf valoftype.intro votTMIIpreserved apply fastforce
+    apply (metis VOT valBij2 val_of_type.simps validClosedTMII)
+    apply (metis VOT valBij2 val_of_type.simps validClosedTMII)
+    done
+
+lemma homVdef:
+  "(\<forall>k. (\<not>wf k \<or> type_of_val k \<noteq> dom_ty homV) \<longrightarrow> (selectImpl homV k) = val_of_type (ran_ty homV))"
+proof rule
+  fix k
+  show "(\<not>wf k \<or> type_of_val k \<noteq> dom_ty homV) \<longrightarrow> (selectImpl homV k) = val_of_type (ran_ty homV)"
+    apply simp
+    apply (cases k rule: ValnCases)
+    apply (simp add: valBij2)
+    using votTMIIpreserved apply auto[1]
+    apply (simp add: votTMIIpreserved)
+    using votTMIIpreserved apply force
+    using votTMIIpreserved apply force
+    apply (simp add: valBij2)+
+    done
+qed
+
+lemma "wf homV" using wff vhomVwfSelect wf.simps[of homV] homVdef by auto
+
+end  (* valoftype locale *)
+
+
+subsubsection \<open>Some more general wf properties\<close>
+
+(* conclude Isabelle type from key of a select assuming wf and typed *)
+lemma
+  assumes "wf (MapV (Inl (FunL f tk tv)))"
+  assumes "wf k"
+  assumes "type_of_val k = dom_ty (MapV (Inl (FunL f tk tv)))"
+  shows "\<exists>k'. toVal3210 k = Inr ( k')"
+proof -
+  have "tmap_lvl (type_of_val (MapV (Inl (FunL f tk tv)))) = 3"
+    using InlC3 wf.simps assms(1) toVal3210.simps wf_impl_wf_ty by force
+  then have "tmap_lvl (dom_ty (MapV (Inl (FunL f tk tv)))) \<le> 2"
+    by auto
+  then have "tmap_lvl (type_of_val k) \<le> 2" using assms by auto
+  then show ?thesis using assms(2) wf_impl_wf_ty
+    by (metis InlC3 One_nat_def Suc_1 Suc_n_not_le_n numeral_3_eq_3 old.sum.exhaust)
+qed
+
+
+text \<open>wf maps are mapval\<close>
+(* see if it works *)
+lemma "mapval_ty (Abs_wf_maps (Inr (Inr mAdd1))) = (TT, TT)"
+  by (simp add: Abs_wf_maps_inverse wf_map_set_def wf_vAdd1)
+
+(* lifted mapval_ty *)
+lemma "mapval_ty (Abs_wf_maps (Inr (Inr mAdd1))) = ((TPrim TInt), (TPrim TInt))"
+  by (simp add: Abs_wf_maps_inverse wf_map_set_def wf_vAdd1)
+
+end
